elle/ElleTest.thy
@@ -1,0 +1,199 @@
+theory ElleTest
+  imports Main String ElleCompiler "ElleCorrect/Valid4"
+begin
+
+(* This file is now all about trying to output code *)
+(* In order to run this from a shell script we need a makefile *)
+value "''ABC''"
+
+definition test1 :: string where
+"test1 = ''DEFG''"
+
+value "test1"
+
+
+(* tests copied from example/LLLL.thy *)
+value "ll_pass1 (ll1.LSeq [ll1.LLab 0, ll1.L (Arith ADD)])"
+value "(inst_size (Arith ADD))"
+
+value "ll_get_node ((0,0), ((llt.LSeq () [((0,0),llt.LLab () 0), ((0,0),llt.LLab () 1)]))::ll2t) [1]"
+value "ll3_init (ll_pass1 (ll1.LSeq [ll1.LLab 0])) :: ll3"
+
+value "(ll3_init (ll_pass1 (ll1.LSeq [ll1.LLab 0])))"
+value "ll3_assign_label (ll3_init (ll_pass1 (ll1.LSeq [ll1.LLab 0])))"
+value "ll3_assign_label (ll3_init (ll_pass1 (ll1.LSeq [ll1.LSeq [ll1.LLab 0], ll1.LSeq [], ll1.LSeq [ll1.LLab 1]])))"
+
+definition prog1 where
+  "prog1 = ll3_assign_label (ll3_init (ll_pass1 (ll1.LSeq [ll1.LLab 0])))"
+value prog1
+
+definition prog2 where
+  "prog2 = ll3_assign_label (ll3_init (ll_pass1 (ll1.LSeq [ll1.L (Arith ADD), ll1.LLab 0])))"  
+  
+value "(case prog2 of
+        Some (_, LSeq _ lsdec) \<Rightarrow> ll3_get_label lsdec [1]
+        | _ \<Rightarrow> None)"
+
+definition src3 where
+"src3 = ll1.LSeq [ll1.LSeq [ll1.LLab 0], ll1.LSeq [ll1.LJmp 1], ll1.LSeq [ll1.LLab 1]]"
+
+definition prog3 where
+"prog3 = ll3_assign_label (ll3_init (ll_pass1 (
+ll1.LSeq [ll1.LSeq [ll1.LLab 0], ll1.LSeq [ll1.LJmp 1], ll1.LSeq [ll1.LLab 1]])))"
+
+value prog3
+
+value "(case prog3 of
+Some p' \<Rightarrow> Some (check_ll3 p')
+| _ \<Rightarrow> None)"
+
+value "(Evm.log256floor 2048) + 1"
+
+value prog3
+
+value "(case prog3 of
+        Some l \<Rightarrow> ll3_resolve_jump_wrap l
+        | _ \<Rightarrow> JFail [666])"
+
+value "(case prog3 of
+        Some (_, LSeq e lsdec) \<Rightarrow> ll3_get_label lsdec e
+        | _ \<Rightarrow> None)"
+  
+value "(case prog3 of
+        Some (_, LSeq _ lsdec) \<Rightarrow> Some (ll3_inc_jump lsdec 0 [1,0])
+        | _ \<Rightarrow> None)"
+
+value "Word.word_rsplit ((Word256.word256FromNat 0) :: 256 word) :: 8 word list" 
+
+value "(case prog3 of
+        Some l \<Rightarrow> process_jumps_loop 40 l
+        | _ \<Rightarrow> None)"
+
+value "(case prog3 of
+        Some l \<Rightarrow> (case (process_jumps_loop 40 l) of
+                       Some l \<Rightarrow> Some (ll4_init l)
+                       | _ \<Rightarrow> None)
+        | _ \<Rightarrow> None)"
+
+
+value "(case prog3 of
+        Some l \<Rightarrow> (case (process_jumps_loop 40 l) of
+                       Some l \<Rightarrow> write_jump_targets [] (ll4_init l)
+                       | _ \<Rightarrow> None)
+        | _ \<Rightarrow> None)"
+(* ll3_resolve_jumps :: "ll3 list \<Rightarrow> ll4 list"*)
+
+value "Word.word_of_int 1 :: 1 word"
+value "Evm.byteFromNat 255"
+
+value "Divides.divmod_nat 255 256"
+
+(* full compiler tests *)
+value "pipeline' src3 20"
+
+value "pipeline src3 20"
+
+definition progif :: ll1 where
+"progif =
+ll1.LSeq [
+ll1.LSeq [
+ll1.L ( Stack (PUSH_N [0])),
+ll1.LJmpI 0,
+ll1.L (Stack (PUSH_N [1])),
+ll1.LJmp 1,
+ll1.LLab 0,
+ll1.L (Stack (PUSH_N [2])),
+ll1.LLab 1
+]]
+"
+
+value "pipeline' progif 30"
+
+(* check of validate_jump_targets
+new question: is validate_jump_targets enough to prove everything we need?
+if so, why were we so concerned about valid3?
+*)
+value "(case (pipeline' progif 30) of
+         None \<Rightarrow> None
+        | Some s \<Rightarrow> Some (ll4_validate_jump_targets [] s))"
+
+value "pipeline progif 30"
+
+definition ll1_sem_test1 where
+"ll1_sem_test1 f i = silly_ll1_sem (ll1.LSeq [ll1.LLab 0, ll1.LJmpI 0]) f (Some) i"
+value "ll1_sem_test1 20 0"
+value "ll1_sem_test1 20 3"
+
+definition ll1_sem_test2 where
+"ll1_sem_test2 f i = silly_ll1_sem
+  (ll1.LSeq [
+    ll1.LSeq [ ll1.LJmpI 0,
+               ll1.L (Arith SUB),
+               ll1.LJmp 1, 
+               ll1.LLab 0,
+               ll1.L (Arith ADD),
+               ll1.LLab 1 ]]) f (Some) i"
+
+value "ll1_sem_test2 100 0"
+value "ll1_sem_test2 100 1"
+value "ll1_sem_test2 100 2"
+
+definition ll1_sem_test2' where
+"ll1_sem_test2' f i = silly_ll1_sem
+  (ll1.LSeq [ll1.LJmpI 0,
+               ll1.L (Arith ADD),
+               ll1.LLab 0]) f (Some) i"
+
+value "ll1_sem_test2' 100 0"
+value "ll1_sem_test2' 100 27"
+
+
+definition ll1_sem_test3 where
+"ll1_sem_test3 f i = silly_ll1_sem
+(ll1.LSeq [ll1.LSeq [ll1.LJmpI 1,
+                     ll1.LLab 0,
+                     ll1.L (Arith SUB),
+                     ll1.LJmpI 1,
+                     ll1.LJmp 0, ll1.LLab 1]]) f Some i"
+value "ll1_sem_test3 120 4"
+value "ll1_sem_test3 120 0"
+
+(* NB *)
+value "ll1_sem_test3 20 15"
+value "ll1_sem_test3 21 15"
+
+(* test to ensure things are being run in correct order,
+as well as check correctness for sequences without labels *)
+definition ll1_sem_test4 where
+"ll1_sem_test4 f i = silly_ll1_sem
+(ll1.LSeq [ll1.L (Arith SUB), ll1.L (Arith ADD)]) f Some i"
+
+value "ll1_sem_test4 10 0"
+value "ll1_sem_test4 10 1"
+
+
+(* ensure invalid jumps crash *)
+definition ll1_sem_test5 where
+"ll1_sem_test5 f i = silly_ll1_sem
+(ll1.LSeq [ll1.LJmpI 0]) f Some i"
+
+value "ll1_sem_test5 10 1"
+
+
+(* semantics tests *)
+value   "elle_sem' (ll1.L (Stack (PUSH_N ([byteFromNat 0]))))
+10 Some (ellest_init 42)"
+
+value  "elle_sem' (ll1.LSeq [ll1.L (Stack (PUSH_N ([byteFromNat 1]))),
+                                   ll1.L (Stack (PUSH_N ([byteFromNat 1]))),
+                                   ll1.L (Arith ADD)])
+10 Some (ellest_init 42)"
+
+value  "program_sem (\<lambda> _ . ()) (prog_init_cctx [Stack (PUSH_N [byteFromNat 0])]) 20 Metropolis
+(InstructionContinue (elle_init_vctx 42))"
+
+value "elle_run (ll1.LSeq [ll1.LLab 0, ll1.L (Stack (PUSH_N [byteFromNat 0]))]) 100"
+value "elle_run (ll1.LSeq [ll1.LLab 0, ll1.L (Stack (PUSH_N [byteFromNat 1])), ll1.LJmpI 0]) 100"
+value "elle_run (ll1.LSeq [ll1.LLab 0, ll1.L (Stack (PUSH_N [byteFromNat 0])) , ll1.LJmpI 0 ]) 100"
+
+end
